LL1/Lemmas.v
@@ -1,0 +1,323 @@
+Require Import List.
+Require Import Lib.Grammar.
+Require Import Lib.ParseTree.
+Require Import Lib.Tactics.
+Require Import LL1.Derivation.
+Require Import LL1.Parser.
+Require Import LL1.ParseTable.
+Import ListNotations.
+
+Lemma eof_fgamma :
+  forall g la gamma,
+    (@first_gamma g) la gamma
+    -> la = EOF
+    -> False.
+Proof.
+  intros g la gamma H.
+  induction H using first_gamma_mutual_ind with
+      (P := fun la x gamma (pf : first_prod la x gamma) =>
+              la = EOF -> False)
+      (P0 := fun la gamma (pf : first_gamma la gamma) =>
+               la = EOF -> False)
+      (P1 := fun la sym (pf : first_sym la sym) =>
+               la = EOF -> False); intros.
+  - apply IHfirst_gamma; trivial.
+  - apply IHfirst_gamma; trivial.
+  - apply IHfirst_gamma; trivial. 
+  - inv H.
+  - apply IHfirst_gamma; trivial.
+Qed.
+
+Lemma nullable_middle_sym :
+  forall g xs ys sym,
+    (@nullable_gamma g) (xs ++ sym :: ys)
+    -> (@nullable_sym g) sym.
+Proof.
+  induction xs; intros.
+  - simpl in H.
+    inv H.
+    auto.
+  - eapply IHxs.
+    inv H.
+    eauto.
+Qed.
+
+Lemma gamma_with_terminal_not_nullable :
+  forall g xs y zs,
+    (@nullable_gamma g) (xs ++ T y :: zs)
+    -> False.
+Proof.
+  induction xs; intros.
+  - simpl in H.
+    inv H.
+  - destruct a.
+    + inv H.
+    + inv H.
+      eapply IHxs; eauto.
+Qed.
+
+Lemma nullable_split :
+  forall g xs ys,
+    (@nullable_gamma g) (xs ++ ys)
+    -> (@nullable_gamma g) ys.
+Proof.
+  induction xs; intros.
+  - auto.
+  - inv H.
+    eapply IHxs; eauto.
+Qed.
+
+Lemma no_first_follow_conflicts :
+  forall tbl g,
+    parse_table_for tbl g
+    -> forall la sym,
+      (@first_sym g) la sym
+      -> (@nullable_sym g) sym
+      -> (@follow_sym g) la sym
+      -> False.
+Proof.
+  intros tbl g Htbl la sym Hfi.
+  destruct Htbl as [Hmin Hcom].
+  induction Hfi using first_sym_mutual_ind with
+      (P := fun la sym gamma
+                (pf : (@first_prod g) la sym gamma) =>
+              (@nullable_prod g) sym gamma
+              -> (@follow_sym g) la sym 
+              -> False)
+      (P0 := fun la gammaSuf
+                 (pf : (@first_gamma g) la gammaSuf) =>
+               forall sym gammaPre,
+                 (@first_prod g) la sym (gammaPre ++ gammaSuf)
+                 -> (@nullable_prod g) sym (gammaPre ++ gammaSuf)
+                 -> (@follow_sym g) la sym
+                 -> False)
+      (P1 := fun la sym (pf : (@first_sym g) la sym) =>
+              (@nullable_sym g) sym
+              -> (@follow_sym g) la sym
+              -> False).
+
+  - intros Hnu Hfo.
+    eapply IHHfi; auto.
+    + assert (gamma = [] ++ gamma) by auto.
+      rewrite H in i.
+      econstructor; eauto.
+    + auto.
+    + auto.
+
+  - intros sym gammaPre Hfi' Hnu Hfo.
+    eapply IHHfi.
+    + inv Hnu.
+      apply nullable_middle_sym in H0.
+      auto.
+    + destruct hd.
+      * inv Hnu.
+        apply gamma_with_terminal_not_nullable in H0.
+        inv H0.
+      * inv Hnu.
+        eapply FoLeft; eauto.
+        assert (NT n :: tl = [NT n] ++ tl) by auto.
+        rewrite H1 in H0.
+        rewrite app_assoc in H0.
+        eapply nullable_split in H0.
+        auto.        
+
+  - intros sym gammaPre Hfi Hnu Hfo.
+    eapply IHHfi; eauto.
+    + assert (NT x :: tl = [NT x] ++ tl) by auto.
+      rewrite H in Hfi.
+      rewrite app_assoc in Hfi.
+      eauto.
+    + rewrite <- app_assoc.
+      simpl.
+      auto.
+
+  - intros Hnu Hfo.
+    inv Hfo.
+
+  - intros Hnu Hfo.
+    inv Hnu.
+    inv H.
+    assert (Hlk : (@lookahead_for g) la (NT x) gamma).
+    { unfold lookahead_for.
+      left.
+      auto. }
+    assert (Hlk' : (@lookahead_for g) la (NT x) ys).
+    { unfold lookahead_for.
+      right.
+      split.
+      { constructor; auto. }
+      { constructor; auto. }}
+    unfold pt_complete in Hcom.
+    apply Hcom in Hlk; apply Hcom in Hlk'.
+    destruct Hlk as [laMap [Hsf Hlf]].
+    destruct Hlk' as [laMap' [Hsf' Hlf']].
+    assert (gamma = ys) by congruence.
+    subst.
+    apply IHHfi.
+    + constructor; auto.
+    + auto.
+Qed.
+
+Lemma lookahead_in_grammar :
+  forall g la x gamma,
+    (@lookahead_for g) la (NT x) gamma
+    -> In (x, gamma) (productions g).
+Proof.
+  intros.
+  destruct H as [Hfi | Hfo].
+  - inv Hfi; auto.
+  - destruct Hfo.
+    inv H; auto.
+Qed.
+
+Lemma gamma_derives_nil_nullable :
+  forall g gamma wpre f wsuf,
+    (@gamma_derives_prefix g) gamma wpre f wsuf
+    -> wpre = nil
+    -> (@nullable_gamma g) gamma.
+Proof.
+  intros g gamma wpre f wsuf Hder.
+  induction Hder using gdp_mutual_ind with
+      (P := fun sym wpre tr wsuf
+                (pf : sym_derives_prefix sym wpre tr wsuf) =>
+              wpre = nil
+              -> nullable_sym sym)
+      (P0 := fun gamma wpre f wsuf
+                 (pf : gamma_derives_prefix gamma wpre f wsuf)
+             =>
+               wpre = nil
+               -> nullable_gamma gamma); intros; subst.
+  - inv H.
+(*  - inv f; simpl in *.
+    eapply eof_fgamma in H2; eauto; inv H2. *)
+  - econstructor.
+    econstructor; eauto.
+    apply lookahead_in_grammar in l; auto.
+  - constructor.
+  - apply app_eq_nil in H; destruct H; subst.
+    destruct hdRoot as [y | x].
+    + inv s.
+    + econstructor; eauto.
+Qed.
+
+Lemma gamma_derives_cons_fg :
+  forall g gamma word f rem,
+    (@gamma_derives_prefix g) gamma word f rem
+    -> forall tok toks,
+      word = tok :: toks
+      -> (@first_gamma g) (LA tok) gamma.
+Proof.
+  intros g gamma word f rem Hder.
+  induction Hder using gdp_mutual_ind with
+      (P := fun sym word tr rem
+                (pf : sym_derives_prefix sym word tr rem) =>
+              forall tok toks,
+                word = tok :: toks
+                -> first_sym (LA tok) sym)
+      (P0 := fun gamma word f rem
+                 (pf : gamma_derives_prefix gamma word f rem)
+             =>
+               forall tok toks,
+                 word = tok :: toks
+                 -> first_gamma (LA tok) gamma); intros; subst.
+  - inv H; constructor.
+  - simpl in *.
+    apply lookahead_in_grammar in l.
+    econstructor.
+    econstructor; eauto.
+  - inv H.
+  - destruct hdRoot.
+    + inv s.
+      inv H.
+      constructor.
+      constructor.
+    + destruct wpre as [| ptok ptoks]; simpl in *.
+      * eapply FiGammaTl.
+        -- inv s; simpl in *.
+           apply lookahead_in_grammar in H1.
+           econstructor.
+           econstructor; eauto.
+           eapply gamma_derives_nil_nullable; eauto.
+        -- eapply IHHder0; eauto.
+      * inv H.
+        eapply FiGammaHd.
+        eapply IHHder; eauto.
+Qed.
+
+Lemma parse_t_ret_leaf :
+  forall tbl y input fuel tree suffix,
+    parse tbl (T y) input fuel = (Some tree, suffix) ->
+    isLeaf tree = true.
+Proof.
+  intros. destruct fuel.
+  - inv H.
+  - simpl in H. destruct input.
+    + inv H.
+    + destruct (Utils.beqString y s).
+      * inv H. reflexivity.
+      * inv H.
+Qed.
+
+Lemma parse_nt_ret_node :
+  forall tbl x input fuel tree suffix,
+    parse tbl (NT x) input fuel = (Some tree, suffix)
+    -> isNode tree = true.
+Proof.
+  intros. destruct fuel.
+  - simpl in H. inv H.
+  - simpl in H. destruct (parseTableLookup x (peek input) tbl).
+    + destruct (parseForest tbl l input fuel). 
+      destruct o. 
+      * inv H. trivial.
+      * inv H.
+    + inv H. 
+Qed.
+
+Lemma tbl_entry_is_lookahead :
+  forall tbl g x la gamma,
+    parse_table_for tbl g
+    -> parseTableLookup x la tbl = Some gamma
+    -> (@lookahead_for g) la (NT x) gamma.
+Proof.
+  intros tbl g x la gamma Htbl Hlkp.
+  destruct Htbl as [Hmin Hcom].
+  unfold pt_minimal in Hmin.
+  unfold parseTableLookup in Hlkp.
+  destruct (StringMap.find x tbl) as [m |] eqn:Hsf.
+  - eapply Hmin; eauto.
+  - inv Hlkp.
+Qed.
+
+Lemma nullable_nonrec :
+  forall g sym,
+    (@nullable_sym g) sym
+    -> exists gamma,
+      (@nullable_prod g) sym gamma
+      /\ ~In sym gamma.
+Proof.
+  intros g sym.
+  induction 1 using nullable_sym_mutual_ind with
+      (P := fun sym gamma (pf : nullable_prod sym gamma) =>
+              exists gamma',
+                (@nullable_prod g) sym gamma'
+                /\ ~In sym gamma')
+      (P0 := fun gamma (pf : nullable_gamma gamma) =>
+               forall sym,
+                 In sym gamma
+                 -> exists gamma',
+                   nullable_prod sym gamma'
+                   /\ ~In sym gamma')
+      (P1 := fun sym (pf : nullable_sym sym) =>
+               exists gamma,
+                 (@nullable_prod g) sym gamma
+                 /\ ~In sym gamma); intros.
+  - destruct (List.In_dec symbol_eq_dec (NT x) ys).
+    + apply IHnullable_sym in i0.
+      eauto.
+    + exists ys.
+      split; auto.
+      constructor; auto.
+  - inv H.
+  - inv H0; eauto.
+  - eauto.
+Qed.
