LL1/Monotonicity.v
@@ -1,73 +1,81 @@
-Require Import List Omega String.
-Require Import Lib.Derivation Lib.Grammar Lib.Lemmas
-               Lib.ParseTree Lib.Tactics.
-Require Import LL1.ParseTable LL1.Parser LL1.Soundness.
+Require Import Arith.
+Require Import Omega.
+Require Import String.
+
+Require Import Lib.Grammar.
+Require Import Lib.ParseTree.
+Require Import Lib.Tactics.
+
+Require Import LL1.Lemmas.
+Require Import LL1.Parser.
+Require Import LL1.ParseTable.
 
 Lemma parse_fuel_monotonic :
-  forall tr tbl sym input suffix fuel fuel2,
-    parse tbl sym input fuel = (Some tr, suffix)
+  forall (tr : tree)
+         (tbl : parse_table)
+         (sym : symbol)
+         (input rem : list string)
+         (fuel fuel2 : nat),
+    parse tbl sym input fuel = (Some tr, rem)
     -> fuel < fuel2
-    -> parse tbl sym input fuel2 = (Some tr, suffix).
+    -> parse tbl sym input fuel2 = (Some tr, rem).
 Proof.
   induction tr as [ s
                   | s f IHparseForest
                   |
                   | tr IHparse f IHparseForest ]
-    using tree_nested_ind with
+                    using tree_nested_ind with
+      
       (P := fun tr =>
-              forall tbl sym input suffix fuel fuel2,
-                parse tbl sym input fuel = (Some tr, suffix)
+              forall tbl sym input rem fuel fuel2,
+                parse tbl sym input fuel = (Some tr, rem)
                 -> fuel < fuel2
-                -> parse tbl sym input fuel2 =
-                   (Some tr, suffix))
+                -> parse tbl sym input fuel2 = (Some tr, rem))
+      
       (Q := fun subtrees =>
-              forall tbl gamma input suffix fuel fuel2,
+              forall tbl gamma input rem fuel fuel2,
                 parseForest tbl gamma input fuel =
-                 (Some subtrees, suffix)
+                 (Some subtrees, rem)
                  -> fuel < fuel2
-                 -> parseForest tbl gamma input fuel2 =
-                    (Some subtrees, suffix)).
+                 -> parseForest tbl gamma input fuel2 = (Some subtrees, rem)).
+
   
-  - intros tbl sym input suffix fuel fuel2 Hparse Hfuel.
+  - (* simplify other bullets to look like this one *)
+    intros tbl sym input rem fuel fuel2 Hparse Hfuel.
+    destruct fuel;  try solve [inv Hparse].
+    destruct fuel2; try solve [inv Hfuel].
+    destruct sym as [y | x].
+    + destruct input as [| token tokens]; try solve [inv Hparse].
+      simpl in *. 
+      destruct (Utils.beqString y token); inv Hparse; auto.
+    + apply parse_nt_ret_node in Hparse; inv Hparse.
+           
+  - intros tbl sym input rem fuel fuel2 Hparse Hfuel.
     destruct fuel.
     + inv Hparse.
     + destruct fuel2.
       * inv Hfuel.
       * destruct sym as [y | x].
-        { destruct input as [| token tokens].
-          { inv Hparse. }
-          { simpl; simpl in Hparse.
-            destruct (Utils.beqString y token).
-            { inv Hparse. reflexivity. }
-            { inv Hparse. }}}
-        { apply parse_nt_ret_node in Hparse. inv Hparse. }
-
-  - intros tbl sym input suffix fuel fuel2 Hparse Hfuel.
-    destruct fuel.
-    + inv Hparse.
-    + destruct fuel2.
-      * inv Hfuel.
-      * destruct sym as [y | x].
-        { apply parse_t_ret_leaf in Hparse. inv Hparse. }
-        { simpl; simpl in Hparse.
-          destruct (parseTableLookup x (peek input) tbl)
+        -- apply parse_t_ret_leaf in Hparse. inv Hparse.
+        -- simpl; simpl in Hparse.
+           destruct (parseTableLookup x (peek input) tbl)
             as [gamma |] eqn:Hlookup.
-          { destruct (parseForest tbl gamma input fuel)
-              as (subresult, input') eqn:Hpf.
-            destruct subresult as [subtrees |].
-            { inv Hparse.
-              apply IHparseForest with (fuel2 := fuel2)in Hpf;
-              clear IHparseForest.
-              { destruct (parseForest tbl gamma input fuel2)
-                  as (subresult, input') eqn:Hpf2.
-                destruct subresult as [subtrees |].
-                { congruence. }
-                { inv Hpf. }}
-              { apply lt_S_n. assumption. }}
-            { inv Hparse. }}
-          { inv Hparse. }}
+           ++ destruct (parseForest tbl gamma input fuel)
+               as (subresult, input') eqn:Hpf.
+              destruct subresult as [subtrees |].
+              ** inv Hparse.
+                 apply IHparseForest with (fuel2 := fuel2)
+                   in Hpf; clear IHparseForest.
+                 --- destruct (parseForest tbl gamma input fuel2)
+                     as (subresult, input') eqn:Hpf2.
+                     destruct subresult as [subtrees |].
+                     +++ congruence.
+                     +++ inv Hpf.
+              --- apply lt_S_n. assumption.
+              ** inv Hparse.
+           ++ inv Hparse.
 
-  - intros tbl gamma input suffix fuel fuel2 Hparse Hfuel.
+  - intros tbl gamma input rem fuel fuel2 Hparse Hfuel.
     destruct fuel.
     + inv Hparse.
     + destruct fuel2.
@@ -87,7 +95,7 @@ Proof.
             { inv Hparse. }}
           { inv Hparse. }}
 
-  - intros tbl gamma input suffix fuel fuel2 Hparse Hfuel.
+  - intros tbl gamma input rem fuel fuel2 Hparse Hfuel.
     destruct fuel.
     + inv Hparse.
     + destruct fuel2.
@@ -145,10 +153,10 @@ Proof.
 Qed.
 
 Lemma parseForest_fuel_monotonic :
-  forall sts tbl gamma input suffix fuel fuel2,
-    parseForest tbl gamma input fuel = (Some sts, suffix)
+  forall sts tbl gamma input rem fuel fuel2,
+    parseForest tbl gamma input fuel = (Some sts, rem)
     -> fuel < fuel2
-    -> parseForest tbl gamma input fuel2 = (Some sts, suffix).
+    -> parseForest tbl gamma input fuel2 = (Some sts, rem).
 Proof.
   induction sts as [ s
                    | s f IHparseForest
@@ -156,20 +164,20 @@ Proof.
                    | tr IHparse f IHparseForest ]
       using forest_nested_ind with
       (P := fun tr =>
-              forall tbl sym input suffix fuel fuel2,
-                parse tbl sym input fuel = (Some tr, suffix)
+              forall tbl sym input rem fuel fuel2,
+                parse tbl sym input fuel = (Some tr, rem)
                 -> fuel < fuel2
                 -> parse tbl sym input fuel2 =
-                   (Some tr, suffix))
+                   (Some tr, rem))
       (Q := fun subtrees =>
-               forall tbl gamma input suffix fuel fuel2,
+               forall tbl gamma input rem fuel fuel2,
                  parseForest tbl gamma input fuel =
-                 (Some subtrees, suffix)
+                 (Some subtrees, rem)
                  -> fuel < fuel2
                  -> parseForest tbl gamma input fuel2 =
-                    (Some subtrees, suffix)).
+                    (Some subtrees, rem)).
   
-  - intros tbl sym input suffix fuel fuel2 Hparse Hfuel.
+  - intros tbl sym input rem fuel fuel2 Hparse Hfuel.
     destruct fuel.
     + inv Hparse.
     + destruct fuel2.
@@ -183,7 +191,7 @@ Proof.
             { inv Hparse. }}}
         { apply parse_nt_ret_node in Hparse. inv Hparse. }
 
-  - intros tbl sym input suffix fuel fuel2 Hparse Hfuel.
+  - intros tbl sym input rem fuel fuel2 Hparse Hfuel.
     destruct fuel.
     + inv Hparse.
     + destruct fuel2.
@@ -208,7 +216,7 @@ Proof.
             { inv Hparse. }}
           { inv Hparse. }}
 
-  - intros tbl gamma input suffix fuel fuel2 Hparse Hfuel.
+  - intros tbl gamma input rem fuel fuel2 Hparse Hfuel.
     destruct fuel.
     + inv Hparse.
     + destruct fuel2.
@@ -228,7 +236,7 @@ Proof.
             { inv Hparse. }}
           { inv Hparse. }}
 
-  - intros tbl gamma input suffix fuel fuel2 Hparse Hfuel.
+  - intros tbl gamma input rem fuel fuel2 Hparse Hfuel.
     destruct fuel.
     + inv Hparse.
     + destruct fuel2.
@@ -286,31 +294,28 @@ Proof.
 Qed. (* Hmm...same proof as the one for parse! *)
 
 Lemma parse_fuel_max :
-  forall fuel tbl sym input fuel2 tr suffix,
-    parse tbl sym input fuel = (Some tr, suffix) ->
-    parse tbl sym input (max fuel fuel2) = (Some tr, suffix).
+  forall fuel tbl sym input fuel2 tr rem,
+    parse tbl sym input fuel = (Some tr, rem) ->
+    parse tbl sym input (max fuel fuel2) = (Some tr, rem).
 Proof.
   intros. 
   pose proof (Max.max_spec fuel fuel2) as H_max_spec.
   destruct H_max_spec.
   - destruct H0. rewrite H1.
-    eapply parse_fuel_monotonic.
-    + eassumption.
-    + assumption.
-  - destruct H0. rewrite H1. assumption.
+    eapply parse_fuel_monotonic; eauto.
+  - destruct H0. rewrite H1. auto.
 Qed.
 
 Lemma parseForest_fuel_max :
-  forall tbl gamma input fuel fuel2 sts suffix,
-    parseForest tbl gamma input fuel = (Some sts, suffix)
+  forall tbl gamma input fuel fuel2 sts rem,
+    parseForest tbl gamma input fuel = (Some sts, rem)
     -> parseForest tbl gamma input (max fuel fuel2) =
-       (Some sts, suffix).
+       (Some sts, rem).
 Proof.
-  intros. pose proof (Max.max_spec fuel fuel2) as H_max_spec.
+  intros.
+  pose proof (Max.max_spec fuel fuel2) as H_max_spec.
   destruct H_max_spec.
   - destruct H0. rewrite H1.
-    eapply parseForest_fuel_monotonic.
-    + eassumption.
-    + assumption.
-  - destruct H0. rewrite H1. assumption.
+    eapply parseForest_fuel_monotonic; eauto.
+  - destruct H0. rewrite H1. auto.
 Qed.
