LL1/ParserTests.v
@@ -8,15 +8,9 @@ Example test1 :
   (Some g311ParseTree1, nil).
 Proof. simpl. reflexivity. Qed.
 
-(* We should be able to parse the empty input string, but
-   there's no way to do this at the moment because the parser
-   requires a lookahead token. I'm going to try to fix this
-   by modifying the parser so that when it encounters an empty 
-   input string, it checks whether the next grammar symbol is
-   a special EOF symbol. *)
 Definition x_y_grammar :=
   [(NT "x", [NT "y"]);
-     (NT "y", [])].
+   (NT "y", [])].
 
 Definition x_map := 
   LookaheadMap.add 
